src/cbor/raw/pulse/CBOR.Pulse.Raw.Read.fst
@@ -252,3 +252,161 @@ ensures exists* a p i' q .
   res
 }
 ```
+
+```pulse
+ghost
+fn cbor_match_map_elim
+  (c: cbor_map)
+  (p: perm)
+  (r: raw_data_item { Map? r })
+  requires
+    cbor_match_map p c r
+  ensures exists* s . 
+    A.pts_to c.cbor_map_ptr #(p `perm_mul` c.cbor_map_array_perm) s **
+    PM.seq_list_match s (Map?.v r) (cbor_match_map_entry (p `perm_mul` c.cbor_map_payload_perm)) **
+    trade
+      (A.pts_to c.cbor_map_ptr #(p `perm_mul` c.cbor_map_array_perm) s **
+        PM.seq_list_match s (Map?.v r) (cbor_match_map_entry (p `perm_mul` c.cbor_map_payload_perm)))
+      (cbor_match_map p c r) **
+    pure (c.cbor_map_length == Map?.len r)
+{
+  unfold (cbor_match_map p c r);
+  with s . assert (A.pts_to c.cbor_map_ptr #(p `perm_mul` c.cbor_map_array_perm) s);
+  ghost
+  fn aux (_: unit)
+    requires emp ** (A.pts_to c.cbor_map_ptr #(p `perm_mul` c.cbor_map_array_perm) s **
+        PM.seq_list_match s (Map?.v r) (cbor_match_map_entry (p `perm_mul` c.cbor_map_payload_perm)))
+    ensures cbor_match_map p c r
+  {
+    fold (cbor_match_map p c r)
+  };
+  Trade.intro _ _ _ aux
+}
+```
+
+let cbor_map_iterator
+= cbor_raw_iterator cbor_map_entry cbor_serialized_map_iterator
+
+let cbor_map_iterator_match
+= cbor_raw_iterator_match
+    cbor_match_map_entry
+    cbor_serialized_map_iterator_match
+
+```pulse
+fn cbor_map_iterator_init
+  (fits: squash (SZ.fits_u64))
+  (c: cbor_raw)
+  (#pm: perm)
+  (#r: Ghost.erased raw_data_item { Map? r })
+requires
+    (cbor_match pm c r)
+returns res: cbor_map_iterator
+ensures exists* p .
+      cbor_map_iterator_match p res (Map?.v r) **
+      trade
+        (cbor_map_iterator_match p res (Map?.v r))
+        (cbor_match pm c r)
+{
+  cbor_match_cases c;
+  match c {
+    CBOR_Case_Serialized_Map c' -> {
+      Trade.rewrite_with_trade
+        (cbor_match pm c r)
+        (cbor_match_serialized_map c' pm r);
+      let i' = cbor_serialized_map_iterator_init c';
+      with p . assert (cbor_serialized_map_iterator_match p i' (Map?.v r));
+      Trade.trans
+        (cbor_serialized_map_iterator_match p i' (Map?.v r))
+        (cbor_match_serialized_map c' pm r)
+        (cbor_match pm c r);
+      let i : cbor_map_iterator = CBOR_Raw_Iterator_Serialized i';
+      Trade.rewrite_with_trade
+        (cbor_serialized_map_iterator_match p i' (Map?.v r))
+        (cbor_map_iterator_match p i (Map?.v r));
+      Trade.trans
+        (cbor_map_iterator_match p i (Map?.v r))
+        (cbor_serialized_map_iterator_match p i' (Map?.v r))
+        (cbor_match pm c r);
+      i
+    }
+    CBOR_Case_Map c' -> {
+      assert_norm (cbor_match pm (CBOR_Case_Map c') (Map (Map?.len r) (Map?.v r)) ==
+        cbor_match_map0 c' pm (Map (Map?.len r) (Map?.v r)) cbor_match
+      );
+      Trade.rewrite_with_trade
+        (cbor_match pm c r)
+        (cbor_match_map0 c' pm r cbor_match);
+      cbor_match_map0_map_trade c' pm r;
+      Trade.trans _ _ (cbor_match pm c r);
+      cbor_match_map_elim c' pm r;
+      with s . assert (A.pts_to c'.cbor_map_ptr #(pm `perm_mul` c'.cbor_map_array_perm) s);
+      Trade.trans
+        (A.pts_to c'.cbor_map_ptr #(pm `perm_mul` c'.cbor_map_array_perm) s **
+          PM.seq_list_match s (Map?.v r) (cbor_match_map_entry (pm `perm_mul` c'.cbor_map_payload_perm)))
+        (cbor_match_map pm c' r)
+        (cbor_match pm c r);
+      let res = cbor_raw_iterator_init_from_array cbor_match_map_entry cbor_serialized_map_iterator_match c'.cbor_map_ptr (SZ.uint64_to_sizet c'.cbor_map_length.value);
+      Trade.trans _ _ (cbor_match pm c r);
+      with p . assert (cbor_raw_iterator_match cbor_match_map_entry cbor_serialized_map_iterator_match p res (Map?.v r));
+      fold (cbor_map_iterator_match p res (Map?.v r));
+      res
+    }
+  }
+}
+```
+
+```pulse
+fn cbor_map_iterator_is_empty
+  (c: cbor_map_iterator)
+  (#pm: perm)
+  (#r: Ghost.erased (list (raw_data_item & raw_data_item)))
+requires
+    cbor_map_iterator_match pm c r
+returns res: bool
+ensures
+    cbor_map_iterator_match pm c r **
+    pure (res == Nil? r)
+{
+  unfold (cbor_map_iterator_match pm c r);
+  let res = cbor_raw_iterator_is_empty
+    cbor_match_map_entry
+    cbor_serialized_map_iterator_match
+    cbor_serialized_map_iterator_is_empty
+    c;
+  fold (cbor_map_iterator_match pm c r);
+  res
+}
+```
+
+```pulse
+fn cbor_map_iterator_next
+  (sq: squash SZ.fits_u64)
+  (pi: R.ref cbor_map_iterator)
+  (#pm: perm)
+  (#i: Ghost.erased cbor_map_iterator)
+  (#l: Ghost.erased (list (raw_data_item & raw_data_item)))
+requires
+    R.pts_to pi i **
+    cbor_map_iterator_match pm i l **
+    pure (Cons? l)
+returns res: cbor_map_entry
+ensures exists* a p i' q .
+    cbor_match_map_entry p res a **
+    R.pts_to pi i' **
+    cbor_map_iterator_match pm i' q **
+    trade
+      (cbor_match_map_entry p res a ** cbor_map_iterator_match pm i' q)
+      (cbor_map_iterator_match pm i l) **
+    pure (Ghost.reveal l == a :: q)
+{
+  unfold (cbor_map_iterator_match pm i l);
+  let res = cbor_raw_iterator_next
+    cbor_match_map_entry
+    cbor_serialized_map_iterator_match
+    (cbor_serialized_map_iterator_next sq)
+    pi;
+  with i' . assert (R.pts_to pi i');
+  fold (cbor_map_iterator_match pm i' (List.Tot.tl l));
+  res
+}
+```
