src/cbor/raw/pulse/everparse/CBOR.Pulse.Raw.Serialized.fst
@@ -157,3 +157,126 @@ fn cbor_serialized_array_iterator_next_cont (_: unit)
 ```
 
 let cbor_serialized_array_iterator_next sq = cbor_raw_serialized_iterator_next _ (jump_raw_data_item sq) cbor_match (cbor_serialized_array_iterator_next_cont ())
+
+let cbor_serialized_map_iterator = cbor_raw_serialized_iterator 
+
+let cbor_serialized_map_iterator_match = cbor_raw_serialized_iterator_match (serialize_nondep_then serialize_raw_data_item serialize_raw_data_item)
+
+module LP = LowParse.Pulse.VCList
+
+```pulse
+ghost
+fn cbor_match_serialized_map_elim
+  (c: cbor_serialized)
+  (pm: perm)
+  (r: raw_data_item { Map? r })
+  requires
+    cbor_match_serialized_map c pm r
+  ensures exists* pm' .
+    pts_to_serialized (LP.serialize_nlist (U64.v (Map?.len r).value) (serialize_nondep_then serialize_raw_data_item serialize_raw_data_item)) c.cbor_serialized_payload #pm' (Map?.v r) **
+    trade
+      (pts_to_serialized (LP.serialize_nlist (U64.v (Map?.len r).value) (serialize_nondep_then serialize_raw_data_item serialize_raw_data_item)) c.cbor_serialized_payload #pm' (Map?.v r))
+      (cbor_match_serialized_map c pm r)
+{
+  unfold (cbor_match_serialized_map c pm r);
+  unfold (cbor_match_serialized_payload_map c.cbor_serialized_payload (pm `perm_mul` c.cbor_serialized_perm) (Map?.v r));
+  with pm' . assert (pts_to_serialized (LP.serialize_nlist (U64.v (Map?.len r).value)  (serialize_nondep_then serialize_raw_data_item serialize_raw_data_item)) c.cbor_serialized_payload #pm' (Map?.v r));
+  ghost fn aux (_: unit)
+    requires emp ** (pts_to_serialized (LP.serialize_nlist (U64.v (Map?.len r).value)  (serialize_nondep_then serialize_raw_data_item serialize_raw_data_item)) c.cbor_serialized_payload #pm' (Map?.v r))
+    ensures (cbor_match_serialized_map c pm r)
+  {
+    fold (cbor_match_serialized_payload_map c.cbor_serialized_payload (pm `perm_mul` c.cbor_serialized_perm) (Map?.v r));
+    fold (cbor_match_serialized_map c pm r);
+  };
+  intro_trade _ _ _ aux
+}
+```
+
+```pulse
+fn cbor_serialized_map_iterator_init
+  (c: cbor_serialized)
+  (#pm: perm)
+  (#r: Ghost.erased raw_data_item { Map? r })
+requires
+    (cbor_match_serialized_map c pm r)
+returns res: cbor_serialized_map_iterator
+ensures
+    (exists* p .
+      cbor_serialized_map_iterator_match p res (Map?.v r) **
+      trade
+        (cbor_serialized_map_iterator_match p res (Map?.v r))
+        (cbor_match_serialized_map c pm r)
+    )
+{
+  cbor_match_serialized_map_elim c pm r;
+  with p . assert (
+    (pts_to_serialized (LowParse.Spec.VCList.serialize_nlist (U64.v (Map?.len (Ghost.reveal r)).value)
+          (serialize_nondep_then serialize_raw_data_item serialize_raw_data_item))
+      c.cbor_serialized_payload
+      #p
+      (Map?.v (Ghost.reveal r)))
+  );
+  let res : cbor_serialized_map_iterator = {
+    s = c.cbor_serialized_payload;
+    len = U64.v (Map?.len r).value;
+  };
+  Trade.rewrite_with_trade
+    (pts_to_serialized (LowParse.Spec.VCList.serialize_nlist (U64.v (Map?.len (Ghost.reveal r)).value)
+          (serialize_nondep_then serialize_raw_data_item serialize_raw_data_item))
+      c.cbor_serialized_payload
+      #p
+      (Map?.v (Ghost.reveal r)))
+    (pts_to_serialized (LowParse.Spec.VCList.serialize_nlist (Ghost.reveal res.len)
+          (serialize_nondep_then serialize_raw_data_item serialize_raw_data_item))
+      res.s
+      #p
+      (Map?.v (Ghost.reveal r))      
+  )
+  ;
+  Trade.trans _ _ (cbor_match_serialized_map c pm r);
+  cbor_raw_serialized_iterator_fold (serialize_nondep_then serialize_raw_data_item serialize_raw_data_item) p res (Map?.v r);
+  Trade.trans _ _ (cbor_match_serialized_map c pm r);
+  fold (cbor_serialized_map_iterator_match p res (Map?.v r));
+  res
+}
+```
+
+let cbor_serialized_map_iterator_is_empty = cbor_raw_serialized_iterator_is_empty _
+
+module LPC = LowParse.Pulse.Combinators
+
+inline_for_extraction
+```pulse
+fn cbor_serialized_map_iterator_next_cont (sq: squash SZ.fits_u64)
+: cbor_raw_serialized_iterator_next_cont #cbor_map_entry #(raw_data_item & raw_data_item) #(and_then_kind parse_raw_data_item_kind parse_raw_data_item_kind) #(nondep_then parse_raw_data_item parse_raw_data_item) (serialize_nondep_then serialize_raw_data_item serialize_raw_data_item) cbor_match_map_entry
+= (x: _) (#pm: _) (#v: _) {
+  let sp = LPC.split_nondep_then
+    serialize_raw_data_item
+    (jump_raw_data_item sq)
+    serialize_raw_data_item
+    x;
+  match sp {
+    SlicePair s1 s2 -> {
+      unfold (LPC.split_nondep_then_post serialize_raw_data_item serialize_raw_data_item x pm v sp);
+      unfold (LPC.split_nondep_then_post' serialize_raw_data_item serialize_raw_data_item x pm v s1 s2);
+      with v1 . assert (pts_to_serialized serialize_raw_data_item s1 #pm v1);
+      with v2 . assert (pts_to_serialized serialize_raw_data_item s2 #pm v2);
+      let res1 = cbor_read s1;
+      let res2 = cbor_read s2;
+      Trade.prod _ (pts_to_serialized serialize_raw_data_item s1 #pm v1) _ (pts_to_serialized serialize_raw_data_item s2 #pm v2);
+      Trade.trans _ _ (pts_to_serialized (serialize_nondep_then serialize_raw_data_item serialize_raw_data_item) x #pm v);
+      let res : cbor_map_entry = {
+        cbor_map_entry_key = res1;
+        cbor_map_entry_value = res2;
+      };
+      Trade.rewrite_with_trade
+        (cbor_match 1.0R res1 v1 ** cbor_match 1.0R res2 v2)
+        (cbor_match_map_entry 1.0R res v);
+      Trade.trans _ _ (pts_to_serialized (serialize_nondep_then serialize_raw_data_item serialize_raw_data_item) x #pm v);
+      res
+    }
+  }
+}
+```
+
+let cbor_serialized_map_iterator_next sq = cbor_raw_serialized_iterator_next _ (jump_nondep_then (jump_raw_data_item sq) (jump_raw_data_item sq)) cbor_match_map_entry (cbor_serialized_map_iterator_next_cont sq)
